PushRelabel.dfy
@@ -11,7 +11,7 @@ module Algorithm {
     const t: nat
     const capacity: array2<nat>
 
-    var flow: array2<nat>
+    var flow: array2<int>
     var height: array<nat>
     var excess: array<int>
 
@@ -31,11 +31,14 @@ module Algorithm {
       requires ValidBucketsStructure()
     {
       -1 <= max_height < 2 * V &&
-      (forall u :: (0 <= u < V && u != s && u != t && excess[u] > 0) ==>
-                     height[u] <= max_height) &&
-      (forall u :: (0 <= u < V && u != s && u != t && excess[u] > 0) ==>
-                     u in buckets[height[u]]) &&
-      (forall h, u :: (0 <= h < 2 * V && 0 <= u < V && u in buckets[h]) ==> height[u] == h)
+      // max_height is the upper bound
+      (forall v :: (0 <= v < V && v!= s && v != t && excess[v] > 0) ==> height[v] <= max_height) &&
+      // If a non terminal node is active it must be in the bucket of its current height
+      (forall v :: (0 <= v < V && v != s && v != t && excess[v] > 0) ==> v in buckets[height[v]]) &&
+      // If a node is in a bucket it must be active and cannot be a terminal node
+      (forall h, v :: (0 <= h < 2 * V && 0 <= v < V && v in buckets[h]) ==> (excess[v] > 0 && v != s && v != t)) &&
+      // If a node is in a bucket it must have the height of that bucket
+      (forall h, v :: (0 <= h < 2 * V && 0 <= v < V && v in buckets[h]) ==> height[v] == h)
     }
 
     predicate ValidStructure()
@@ -53,32 +56,32 @@ module Algorithm {
       reads this, capacity, flow, height, excess, buckets
     {
       ValidStructure() &&
-      FlowGraph.ValidFlow(V, s, t, capacity, flow) &&
-      FlowGraph.ValidPreflow(V, s, t, excess) &&
+      FlowGraph.ValidPreflow(V, s, t, capacity, flow) &&
+      FlowGraph.ValidExcess(V, s, t, capacity, flow, excess) &&
       FlowGraph.ValidLabeling(V, s, t, capacity, flow, height) &&
       ValidBuckets()
     }
 
-    function ResidualCapacity(u: nat, v: nat): nat
+    function ResidualCapacity(v: nat, w: nat): nat
       reads this, capacity, flow
       requires Graph.ValidGraph(V, s, t)
       requires FlowGraph.ValidFlowMatrixShape(V, flow)
       requires FlowGraph.ValidCapacityMatrixShape(V, capacity)
-      requires FlowGraph.ValidFlow(V, s, t, capacity, flow)
-      requires Graph.ValidNode(V, u) && Graph.ValidNode(V, v)
+      requires FlowGraph.ValidPreflow(V, s, t, capacity, flow)
+      requires Graph.ValidNode(V, v) && Graph.ValidNode(V, w)
     {
-      FlowGraph.ResidualCapacity(V, s, t, capacity, flow, u, v)
+      FlowGraph.ResidualCapacity(V, s, t, capacity, flow, v, w)
     }
 
-    method Push(u: nat, v: nat)
+    method Push(v: nat, w: nat)
       requires Valid()
 
       // Preconditions for a valid push:
-      requires Graph.ValidNode(V, u) && Graph.ValidNode(V, v)   // u and v must be nodes in the Graph
-      requires !FlowGraph.NodeIsSourceOrSink(u, s, t)           // u cannot be equal to the source or sink
-      requires FlowGraph.NodeIsActive(V, u, excess)             // u must be active
-      requires ResidualCapacity(u, v) > 0                       // There must be pipe space
-      requires height[u] == height[v] + 1                       // Water must flow exactly one step downhill
+      requires Graph.ValidNode(V, v) && Graph.ValidNode(V, w)   // v and w must be nodes in the Graph
+      requires !FlowGraph.NodeIsSourceOrSink(v, s, t)           // v cannot be equal to the source or sink
+      requires FlowGraph.NodeIsActive(V, v, excess)             // w must be active
+      requires ResidualCapacity(v, w) > 0                       // There must be pipe space
+      requires height[v] == height[w] + 1                       // Water must flow exactly one step downhill
 
       // postconditions
       ensures Valid()
@@ -86,50 +89,47 @@ module Algorithm {
       modifies flow, excess, buckets
     {
       // Calculate how much water we can push
-      var push_val := excess[u];
-      var res_cap := ResidualCapacity(u, v);
-      if (res_cap < push_val) {
-        push_val := res_cap;
+      var delta := excess[v];
+      var res_cap := ResidualCapacity(v, w);
+      if (res_cap < delta) {
+        delta := res_cap;
       }
 
-      // Cancel out any backward flow from v to u
-      var cancel_flow := flow[v, u];
-      if (push_val < cancel_flow) {
-        cancel_flow := push_val;
+      label BeforeMutation:
+      flow[v, w] := flow[v, w] + delta;
+      flow[w, v] := flow[w, v] - delta;
+      FlowGraph.LemmaFlowSumAfterPush@BeforeMutation(V, flow, v, w, delta, V);
+
+      // Store w's inital active state far later use
+      var old_w_active := FlowGraph.NodeIsActive(V, w, excess);
+
+      excess[v] := excess[v] - delta;
+      excess[w] := excess[w] + delta;
+
+      if (excess[v] == 0) {
+        buckets[height[v]] := buckets[height[v]] - {v};
       }
-      flow[v, u] := flow[v, u] - cancel_flow;
-
-      // Push the remaining amount forward from u to v
-      var forward_push := push_val - cancel_flow;
-      flow[u, v] := flow[u, v] + forward_push;
-
-      // Store v's inital active state far later use
-      var old_v_active := FlowGraph.NodeIsActive(V, v, excess);
-
-      // Update the excess arrays
-      excess[u] := excess[u] - push_val;
-      excess[v] := excess[v] + push_val;
 
       // Update the Highest-Label Buckets
-      // If v was NOT active, and is not s or t (which implies it is active now), it enters the buckets.
-      if (!old_v_active && !FlowGraph.NodeIsSourceOrSink(v, s, t)) {
-        assert FlowGraph.NodeIsActive(V, v, excess);
+      // If w was NOT active and w is not s or t, which implies it is active now, it enters the buckets.
+      if (!old_w_active && !FlowGraph.NodeIsSourceOrSink(w, s, t)) {
+        assert FlowGraph.NodeIsActive(V, w, excess);
 
-        buckets[height[v]] := buckets[height[v]] + {v};
+        buckets[height[w]] := buckets[height[w]] + {w};
         // We don't need to update max_height here because water flows downhill
-        // height[v] is strictly less than height[u], so it cannot become the new max_height.
+        // height[w] is strictly less than height[v], so it cannot become the new max_height.
       }
     }
 
-    method Relabel(u: nat)
+    method Relabel(v: nat)
       requires Valid()
 
       // Preconditions for a valid relabel:
-      requires Graph.ValidNode(V, u)                  // u must be a node in the Graph
-      requires !FlowGraph.NodeIsSourceOrSink(u, s, t) // u cannot be equal to the source or sink
-      requires FlowGraph.NodeIsActive(V, u, excess)   // u must be active
-      // u cannot be relabeled if it has a downhill neighbor
-      requires forall v :: 0 <= v < V && ResidualCapacity(u, v) > 0 ==> height[u] <= height[v]
+      requires Graph.ValidNode(V, v)                  // v must be a node in the Graph
+      requires !FlowGraph.NodeIsSourceOrSink(v, s, t) // v cannot be equal to the source or sink
+      requires FlowGraph.NodeIsActive(V, v, excess)   // v must be active
+      // v cannot be relabeled if it has a downhill neighbor
+      requires forall w :: 0 <= w < V && ResidualCapacity(v, w) > 0 ==> height[v] <= height[w]
 
       // Postconditions
       ensures Valid()
@@ -137,76 +137,68 @@ module Algorithm {
       modifies this, height, buckets
     {
       // Find the lowest neighbor in the residual graph
-      // We initialize minHeightNeighbourOfU to an impossibly high value (2 * V)
-      var minHeightNeighbourOfU: nat := 2 * V;
-      var v := 0;
+      // We initialize minHeightNeighbour to an impossibly high value (2 * V)
+      var minHeightNeighbour: nat := 2 * V;
+      var w := 0;
+      while (w < V)
+        invariant 0 <= w <= V
+        invariant minHeightNeighbour <= 2 * V
+        invariant forall k :: 0 <= k < w && ResidualCapacity(v, k) > 0 ==> minHeightNeighbour <= height[k]
 
-      while (v < V)
-        invariant 0 <= v <= V
-        invariant minHeightNeighbourOfU <= 2 * V
-        invariant forall k :: 0 <= k < v && ResidualCapacity(u, k) > 0 ==> minHeightNeighbourOfU <= height[k]
-
-        // Because u had no downhill neighbors, height[u] MUST be <= minHeightNeighbourOfU.
+        // Because v had no downhill neighbors, height[v] MUST be <= minHeightNeighbour.
         // invariant so that Dafny does not forget
-        invariant height[u] <= minHeightNeighbourOfU
+        invariant height[v] <= minHeightNeighbour
       {
-        if (ResidualCapacity(u, v) > 0) {
-          if (height[v] < minHeightNeighbourOfU) {
-            minHeightNeighbourOfU := height[v];
+        if (ResidualCapacity(v, w) > 0) {
+          if (height[w] < minHeightNeighbour) {
+            minHeightNeighbour := height[w];
           }
         }
-        v := v + 1;
+        w := w + 1;
       }
-      // Assert minHeightNeighbourOfU is actual minimum
-      assert forall k :: 0 <= k < V && ResidualCapacity(u, k) > 0 ==> minHeightNeighbourOfU <= height[k];
+      // Assert minHeightNeighbour is actual minimum
+      assert forall k :: 0 <= k < V && ResidualCapacity(v, k) > 0 ==> minHeightNeighbour <= height[k];
 
-      // Prove a path to the source exists from u
-      FlowGraph.Lemma_ActiveNodeHasPathToSource(V, s, t, capacity, flow, excess, u);
+      // ------ Lemma's and proofs needed to prove height[v] < 2 * V after relabel ------
+      // Prove a path to source exists from v
+      FlowGraph.Lemma_ActiveVertexHasPathToSource(V, s, t, capacity, flow, excess, v);
       // Extract that path
-      ghost var pathToSource :| FlowGraph.IsSimpleResidualPath(V, s, t, capacity, flow, pathToSource) && pathToSource[0] == u && pathToSource[|pathToSource|-1] == s;
+      ghost var pathToSource :| FlowGraph.IsSimpleResidualPath(V, s, t, capacity, flow, pathToSource) && pathToSource[0] == v && pathToSource[|pathToSource|-1] == s;
 
-      // Since u != s, the path has at least 2 nodes. Grab the next node in the path
+      // Since v != s, the path has at least 2 nodes. Grab the next node in the path
       assert |pathToSource| >= 2;
       ghost var pathToSourceNextNode := pathToSource[1];
 
-      // Because u and path_v are connected on a residual path, there is residual capacity
-      assert FlowGraph.ResidualCapacity(V, s, t, capacity, flow, u, pathToSourceNextNode) > 0;
+      // Because v and pathToSourceNextNode are connected on a residual path, there is residual capacity
+      assert FlowGraph.ResidualCapacity(V, s, t, capacity, flow, v, pathToSourceNextNode) > 0;
 
-      // get the remainder of the path (from path_v to s)
-      ghost var pathToSourceWithoutU := pathToSource[1..];
+      // get the remainder of the path (from pathToSourceNextNode to s)
+      ghost var pathToSourceWithoutV := pathToSource[1..];
 
       // Apply length and telescoping height lemmas
       Graph.Lemma_SimplePathHasBoundedLength(V, pathToSource);
       assert |pathToSource| <= V;
-      FlowGraph.Lemma_PathTelescopingHeight(V, s, t, capacity, flow, height, pathToSourceWithoutU);
-      assert height[pathToSourceNextNode] <= height[s] + |pathToSourceWithoutU| - 1;
-      // Since |pathToSource| <= V, the subpath has length <= V - 1
-      assert |pathToSourceWithoutU| <= V - 1;
-      // Since height[s] == V, we get:
-      assert height[pathToSourceNextNode] <= V + (V - 1) - 1;
+      FlowGraph.Lemma_PathTelescopingHeight(V, s, t, capacity, flow, height, pathToSourceWithoutV);
+      assert height[pathToSourceNextNode] <= height[s] + |pathToSourceWithoutV| - 1;
+      assert height[pathToSourceNextNode] <= V + (V - 1) - 1; // Since height[s] == V && ((|pathToSource| <= V) ==> (|pathToSourceWithoutV| <= V - 1))
       assert height[pathToSourceNextNode] <= 2 * V - 2;
       assert height[pathToSourceNextNode] < 2 * V - 1;
 
-      // This proves there exists a path to source where
-      // - height[pathToSourceNextNode] < 2 * V - 1
-      // minHeightNeighbourOfU is the neighbour on the path where the next node has the minimum height
-      // this means the following assertion also holds
-      assert minHeightNeighbourOfU < 2 * V - 1;
+      // This proves there exists a path to source where height[pathToSourceNextNode] < 2 * V - 1
+      // minHeightNeighbour is the neighbour on the path where the next node has the minimum height
+      // this means the following assertions also holds
+      assert minHeightNeighbour < 2 * V - 1;
+      assert minHeightNeighbour + 1 < 2 * V;
+      // ------------
 
-      // Remove u from its old bucket
-      buckets[height[u]] := buckets[height[u]] - {u};
+      buckets[height[v]] := buckets[height[v]] - {v};
 
-      // Update u's height
-      height[u] := minHeightNeighbourOfU + 1;
-      // from these above lemmas we can thus conclude that height[u] falls within the bounds of the buckets
-      assert height[u] < 2 * V;
+      height[v] := minHeightNeighbour + 1;
 
-      // Add u to its new, higher bucket
-      buckets[height[u]] := buckets[height[u]] + {u};
+      buckets[height[v]] := buckets[height[v]] + {v};
 
-      // Because we lifted a node, it might be the new absolute highest active node
-      if (height[u] > max_height) {
-        max_height := height[u];
+      if (height[v] > max_height) {
+        max_height := height[v];
       }
     }
   }
